NEW : added set content, installation instructions and did some changes in the discrete math folder

Content/Discrete_Math/Algorithms.lean
@@ -5,110 +5,97 @@ Author: Yves Jäckle.
 -/
 
 import Mathlib.Tactic
-import Mathlib.Data.List.Sort
 
 
-/-- Inserting x into list L at the first entry where it's smaller-/
-def my_insert (x : ℕ) : List ℕ → List ℕ
-| [] => [x]
-| y :: l =>
-    if x ≤ y
-    then x :: (y :: l)
-    else y :: (my_insert x l)
+-- # Lists and algorithms on lists
 
-/-- `y` is in the list obtained by inserting `x` into `l` iff it is either `x` or it is in `l` -/
-lemma mem_insertion (x y: ℕ) (l : List ℕ) : y ∈ my_insert x l ↔ (y = x ∨ y ∈ l) :=
-  by
-  constructor
-  · induction' l with z l ih
-    · dsimp [my_insert]
-      rw [List.mem_singleton]
-      apply Or.inl
-    · intro H
-      dsimp [my_insert] at H
-      split_ifs at H with Q
-      · rw [List.mem_cons] at H
-        exact H
-      · rw [List.mem_cons] at H
-        cases H with
-        | inl lef =>
-            right
-            rw [lef]
-            exact List.mem_cons_self z l
-        | inr rig =>
-            specialize ih rig
-            cases ih with
-            | inl a =>
-                left
-                exact a
-            | inr b =>
-                right
-                exact List.mem_cons_of_mem z b
-  · induction' l with z l ih
-    · dsimp [my_insert]
-      rw [List.mem_singleton]
-      intro h
-      cases h with
-      | inl a => exact a
-      | inr b => contradiction
-    · intro H
-      dsimp [my_insert]
-      split_ifs with Q
-      · cases H with
-        | inl a =>
-            rw [a]
-            exact List.mem_cons_self x (z :: l)
-        | inr b =>
-            exact List.mem_cons_of_mem x b
-      · cases H with
-        | inl a =>
-            apply List.mem_cons_of_mem z
-            apply ih
-            left
-            exact a
-        | inr b =>
-            rw [List.mem_cons] at b
-            cases b with
-            | inl c =>
-              rw [c]
-              exact List.mem_cons_self z (my_insert x l)
-            | inr d =>
-                apply List.mem_cons_of_mem z
-                apply ih
-                right
-                exact d
+-- ### Class
 
-/-- If list `l` is sorted, then using `my_insert` to insert some number maintains this property -/
-lemma insertion_maintains_sort (x: ℕ) (l : List ℕ) (hl : List.Sorted Nat.le l) :
-  List.Sorted Nat.le (my_insert x l) :=
-  by
-  induction' l with y l ih
-  · dsimp [my_insert]
-    exact List.sorted_singleton x
-  · dsimp [my_insert]
-    split_ifs with H
-    · rw [List.sorted_cons]
-      constructor
-      · intro z z_def
-        rw [List.mem_cons] at z_def
-        cases z_def with
-          | inl lef =>
-              rw [lef]
-              apply H
-          | inr rig =>
-              rw [List.sorted_cons] at hl
-              apply le_trans H
-              exact hl.left z rig
-      · exact hl
-    · push_neg at H
-      rw [List.sorted_cons] at *
-      constructor
-      · intro z z_def
-        rw [mem_insertion] at z_def
-        cases z_def with
-        | inl a =>
-            rw [a]
-            exact le_of_lt H
-        | inr b =>
-            exact hl.left z b
-      · exact ih hl.right
+#check [1,2,3,4]
+
+#check 1 :: 2 :: 3 :: 4 :: []
+
+#check List.cons 1 (List.cons 2 (List.cons 3 (List.cons 4 [])))
+
+
+def length : List α → ℕ
+| [] => 0
+| _ :: l => 1 + length l
+
+#eval length [4,2,3,7]
+
+#check List.length
+
+
+def concat : List α → List α → List α
+| [], l => l
+| x :: l , L => List.cons x (concat l L)
+
+#eval concat [1,2] [3,4]
+
+#check List.append
+#eval [1,2] ++ [3,4]
+
+example (l : List ℕ) : concat l [] = l := by
+  induction' l with x l ih
+  · unfold concat
+    rfl
+  · unfold concat
+    rw [ih]
+
+
+def map (f : ℕ → ℕ) : List ℕ → List ℕ
+| [] => []
+| x :: l => f x :: (map f l)
+
+#eval map (fun x : ℕ => x^2) [1,2,5]
+
+#check List.map
+#eval [1,2,5].map (· ^2)
+
+example (l : List ℕ) (f : ℕ → ℕ): length (map f l) = length l := by
+  induction' l with x l ih
+  · unfold map
+    rfl
+  · unfold map
+    unfold length
+    rw [ih]
+
+
+def get (l : List ℕ) (i : ℕ) (wow : i < l.length): ℕ :=
+  match l with
+  | [] => (by exfalso ; rw [List.length_nil] at wow ; apply Nat.not_lt_zero _ wow )
+  | x :: xs => match i with
+              | 0 => x
+              | n+1 => get xs n (by rw [List.length_cons] at wow ; apply Nat.lt_of_add_lt_add_right wow )
+
+#eval get [7,8,9] 1 (by decide)
+
+
+-- ### Exercise
+
+#check List.sublists
+
+#check List.length_sublists
+
+def sublists : List α → List (List α)
+| [] => [[]]
+| x :: l => (sublists l) ++ ((sublists l).map (List.cons x))
+
+#eval sublists [1,2,3]
+
+example (l : List α) : List.length (sublists l) = 2 ^ List.length l := by
+  induction' l with x l ih
+  · unfold sublists
+    rw [List.length_singleton]
+    rw [List.length_nil]
+    norm_num
+  · unfold sublists
+    rw [List.length_append]
+    rw [List.length_map]
+    rw [ih]
+    rw [List.length_cons]
+    rw [Nat.succ_eq_add_one]
+    rw [pow_add]
+    rw [pow_one]
+    rw [mul_two]
