Content/Logic_Functions_Sets/Solutions_Sets_Basics.lean
@@ -1,0 +1,103 @@
+
+import Mathlib.Tactic
+
+
+-- # Sets, basics
+
+
+-- ### Syntax
+
+
+def IsEven (n : ℕ) : Prop :=
+  ∃ t, n = 2 * t
+
+#check {n : ℕ | IsEven n}
+
+example : 74 ∈ {n : ℕ | IsEven n} := by
+  use 37
+
+example : 74 ∈ {n : ℕ | IsEven n} := by
+  rw [Set.mem_def]
+  use 37
+
+
+
+-- ### Operations
+
+variable (X : Type) (A B C D : Set X)  (x : X)
+
+
+example : A ⊆ B ↔ ∀ x, x ∈ A → x ∈ B := by
+  rfl
+
+#check Set.subset_def
+
+
+example : x ∈ A ∪ B ↔ x ∈ A ∨ x ∈ B := by
+  rfl
+
+#check Set.mem_union
+
+#check Set.mem_inter
+
+
+example : x ∈ (Set.univ : Set X) := by
+  apply Set.mem_univ
+
+example : x ∈ (∅ : Set X) → False := by
+  rw [Set.mem_empty_iff_false]
+  trivial
+
+
+example : x ∉ A → x ∈ A → False := by
+  intro h
+  exact h
+
+example : x ∈ A → x ∉ A → False := by
+  intro h1 h2
+  exact h2 h1
+
+
+example : x ∉ (∅ : Set X) := by
+  intro h
+  exact h
+
+example : x ∈ Aᶜ ↔ x ∉ A := by rfl
+
+example : A ⊆ B → B ⊆ A → A = B := by
+  intro hAB hBA
+  ext x
+  constructor
+  · intro h
+    apply hAB
+    exact h
+  · intro h
+    apply hBA
+    exact h
+
+
+-- ### Exercises
+
+example : A ⊆ B → A ⊆ C → A ⊆ B ∩ C := by
+  intro hAB hAC x hxA
+  constructor
+  · apply hAB
+    exact hxA
+  · exact hAC hxA
+
+example : B ⊆ A → C ⊆ A → B ∪ C ⊆ A :=
+  by
+  rintro hBA hCA x (hxB | hxC)
+  · exact hBA hxB
+  · exact hCA hxC
+
+example : ∅ ⊆ A := by
+  intro x hx
+  rw [Set.mem_empty_iff_false] at hx
+  exfalso
+  exact hx
+
+example : A ⊆ B → x ∉ B → x ∉ A := by
+  intro hAB hB hA
+  apply hB
+  exact hAB hA
